\item {[}ALVL/2013/P1/9{]}
\begin{enumerate}
\item Prove by the method of mathematical induction that 
\[
\sum_{r=1}^{n}r\left(2r^{2}+1\right)=\frac{1}{2}n\left(n+1\right)\left(n^{2}+n+1\right).
\]
 \hfill{}{[}5{]}
\item It is given that $f\left(r\right)=2r^{3}+3r^{2}+r+24$. Show that
\[
f(r)-f(r-1)=ar^{2},
\]
for a constant $a$ to be determined. Hence find a formula for $\sum_{r=1}^{n}r^{2}$,
fully factorising your answer. \hfill{} {[}5{]}
\item Find $\sum_{r=1}^{n}f\left(r\right)$. (You should not simplify your
answer.) \hfill{} {[}3{]}
\end{enumerate}
